---
title: "CHE 318 Lecture 03"
subtitle: "Molecular Diffusion in Gases: General Solutions"
author: "Dr. Tian Tian"
date: "2026-01-09"
format:
  html: {}
  revealjs:
    output-file: slides.html
---

::: {.content-visible when-format="html" unless-format="revealjs"}

::: {.callout-note}
Slides üëâ  [Open presentationüóíÔ∏è](./slides.html)
:::

:::

## Recap

- **Governing equation** for diffusion binary mixture gas systems
$$
N_{A} = -c_T D_{AB} \dfrac{d x_A}{dz} + x_A(N_A + N_B)
$$

::: {.columns}
::: {.column width="50%"}
- Case 1: equimolar counter diffusion (EMCD)
  - $N_A + N_B = 0$
  - $N_A = -c_T D_{AB} \dfrac{d x_A}{d z}$
  - Linear $x_A$, $c_A$ and $p_A$ profiles
  - $N_A = \dfrac{D_{AB}}{RT(z_2 - z_1)}(p_{A1} - p_{A2})$
:::
::: {.column width="50%"}
- Case 2: diffusion through stagnant B
  - $N_B = 0$
  - $N_A(1 - x_A) = -c_T D_{AB}\dfrac{d x_A}{dz}$
  - Usually in log-mean pressure form
  - $N_A = \dfrac{D_{AB}}{RT(z_2-z_1)}
  \dfrac{p_T}{p_{Bm}} \left(p_{A1} - p_{A2}\right)
$
:::
:::

---

## Office Hour

- Wednesday 11:15 - 12:15
- DICE 12-245
- Can take place in other meeting rooms if many people are attending
- Please use seminar time wisely for assignment questions!

## Learning Outcomes {.center}

After today's lecture, you will be able to:

- **Derive** general solution for mass transport in binary gas mixture
- **Define** the conditions for each cases we have studied so far
- **Formulate** governing equations for various case systems
- **Apply** general solution to defined problem
- **Analyze** pressure / concentration profile

## Deriving the General Solution (I)

General case for steady state (S.S) transport

- $N_B = k N_A$ ($k$ is a constant. *why?*)
- Only $x_A$ (or $c_A$, $p_A$) dependent on $z$, not $N_A$ or $N_B$ üëâ separation of variables!

```{=tex}
\begin{align}
N_A - x_A(N_A + N_B) &= -D_{AB}c_T \dfrac{d x_A}{dz}\\
\frac{dz}{D_{AB} c_T} &= -\dfrac{dx_A}{N_A - x_A (N_A + N_B)} \\
\int_{z_1}^{z_2} \frac{dz}{D_{AB} c_T} &= \int_{x_{A1}}^{x_{A2}} -\dfrac{dx_A}{N_A - x_A (N_A + N_B)}
\end{align}
```

## Deriving the General Solution (II)
- L.H.S.

$$
\int_{z_1}^{z_2} \frac{dz}{D_{AB} c_T} = \frac{(z_2 - z_1)}{D_{AB} c_T}
$$

- R.H.S.

Using substitution $u = N_A - x_A (N_A + N_B)$, $d u = -(N_A + N_B)\,dx_A$

```{=tex}
\begin{align}
\int_{x_{A1}}^{x_{A2}} -\dfrac{dx_A}{N_A - x_A (N_A + N_B)}
&= - \cdot - \frac{1}{N_A + N_B} \ln\!\left[N_A - x_A (N_A + N_B)\right] \bigg\vert_{x_{A1}}^{x_{A2}} \\
&= \frac{1}{N_A + N_B} \ln\!\left[\dfrac{
N_A - x_{A2} (N_A + N_B)}
{N_A - x_{A1} (N_A + N_B)}
\right]
\end{align}
```

## Deriving the General Solution (III)

We want to solve for $N_A$

```{=tex}
\begin{align}
\frac{(z_2 - z_1)}{c_T D_{AB}}
&= \frac{1}{N_A + N_B} \ln\!\left[\dfrac{
N_A - x_{A2} (N_A + N_B)}
{N_A - x_{A1} (N_A + N_B)}
\right] \\
N_A &= \frac{c_T D_{AB}}{(z_2 - z_1)}
\frac{N_A}{N_A + N_B} \ln\!\left[\dfrac{
N_A - x_{A2} (N_A + N_B)}
{N_A - x_{A1} (N_A + N_B)}
\right]
\end{align}
```

We can gather all $N_A / (N_A + N_B)$ in the R.H.S since it's a constant

```{=tex}
\begin{align}
\boxed{
N_A = \frac{ c_T D_{AB}}{(z_2 - z_1)}
\left(\frac{N_A}{N_A + N_B}\right)

\ln\!\left[\dfrac{
\frac{N_A}{N_A + N_B} - x_{A2}}
{\frac{N_A}{N_A + N_B} - x_{A1}}
\right]
}
\end{align}
```

- This is the general solution for binary gas transport.
- Also works for $N_A = -N_B$ (EMCD), with a little bit trick

## Relation Between Gen. Sol. and EMCD

The general solution is not applicable $N_B = -N_A$, but we can prove $N_B / N_A \to -1$ reduces to the EMCD equation.

- Let $s = N_A / (N_A + N_B)$, so $s \to \infty$ when $N_B/N_A \to -1$
- Use the Taylor expansion that $\lim_{u \to 0} \ln(1-u) = -u$

```{=tex}
\begin{align}
\lim_{s \to \infty} \left(\frac{N_A}{N_A + N_B}\right)

\ln\!\left[\dfrac{
\frac{N_A}{N_A + N_B} - x_{A2}}
{\frac{N_A}{N_A + N_B} - x_{A1}}
\right]

&=

s \ln\!\left(\frac{s - x_2}{s - x_1}\right) \\

&= s \ln\!\left(\frac{1 - x_2/s}{1 - x_1/s}\right) \\
&= s [(-\frac{x_2}{s}) - (-\frac{x_1}{s})] \\
&= x_1 - x_2
\end{align}
```

This **is** the EMCD result!

## Three Forms of Gass Mass Transport Equations (I)

In $c_A$ form

::: {.columns}
::: {.column width="40%"}
- Case 1: EMCD
  - $N_A + N_B = 0$
  $$
  N_A = \dfrac{D_{AB}}{(z_2 - z_1)}(c_{A1} - c_{A2})
  $$
  
- Case 2: stagnant B
  - $N_B = 0$
  
  $$
  N_A = \frac{D_{AB} c_T }{(z_2 - z_1)}
  \ln\! \left(
  \frac{1 - \frac{c_{A2}}{c_T} }
       {1-\frac{c_{A1}}{c_T}}
  \right)
  $$
  
:::

::: {.column width="60%"}

- General solution

  - $N_B = \lambda N_A$
  
$$
N_A = \frac{D_{AB} c_T}{(z_2 - z_1)} 
\frac{N_A}{N_A + N_B}
\ln\!\left[\dfrac{
\frac{N_A}{N_A + N_B} - \frac{c_{A2}}{c_T}}
{\frac{N_A}{N_A + N_B} - \frac{c_{A1}}{c_T}}
\right]
$$

:::
:::

## Three Forms of Gass Mass Transport Equations (II)

In $x_A$ form

::: {.columns}
::: {.column width="40%"}
- Case 1: EMCD
  - $N_A + N_B = 0$
  $$
  N_A = \dfrac{D_{AB} c_T}{(z_2 - z_1)}(x_{A1} - x_{A2})
  $$
  
- Case 2: stagnant B
  - $N_B = 0$
  
  $$
  N_A = \frac{D_{AB} c_T }{(z_2 - z_1)}
  \ln\! \left(
  \frac{1 - x_{A2} }
       {1- x_{A1}}
  \right)
  $$
  
:::

::: {.column width="60%"}

- General solution

  - $N_B = \lambda N_A$
  
$$
N_A = \frac{D_{AB} c_T}{(z_2 - z_1)} 
\frac{N_A}{N_A + N_B}
\ln\!\left[\dfrac{
\frac{N_A}{N_A + N_B} - x_{A2}}
{\frac{N_A}{N_A + N_B} - x_{A1}}
\right]
$$

:::
:::

## Three Forms of Gass Mass Transport Equations (III)

In $p_A$ form (ideal gas)

::: {.columns}
::: {.column width="40%"}
- Case 1: EMCD
  - $N_A + N_B = 0$
  $$
  N_A = \dfrac{D_{AB}}{RT(z_2 - z_1)}(p_{A1} - p_{A2})
  $$
  
- Case 2: stagnant B
  - $N_B = 0$
  
  $$
  N_A = \frac{D_{AB} p_T}{RT(z_2 - z_1)}
  \ln\! \left(
  \frac{p_T - p_{A2}}
       {p_T - p_{A1}}
  \right)
  $$
  
:::

::: {.column width="60%"}

- General solution

  - $N_B = \lambda N_A$
  
$$
N_A = \frac{D_{AB} p_T}{RT(z_2 - z_1)} 
\frac{N_A}{N_A + N_B}
\ln\!\left[\dfrac{
\frac{N_A}{N_A + N_B} - x_{A2}}
{\frac{N_A}{N_A + N_B} - x_{A1}}
\right]
$$

:::
:::

## General Solution -- $x_A(z)$ Profile

In all the cases we study the S.S. condition:

$$\frac{d N_A}{d z} = 0$$

For the general case $s = N_A / (N_A + N_B)$, we have 

```{=tex}
\begin{align}
\frac{dN_A}{dz} &= \frac{d}{dz} \left[ \frac{D_{AB} c_T}{s - x_A} \frac{d x_A}{d z}\right] = 0\\
\frac{D_{AB} c_T}{s - x_A} \frac{d x_A}{d z} &= \mathrm{Const}
\end{align}
```

$x_A(z)$ has a general solution with exponential form (with $K_1$ and $K_2$ being constants)

```{=tex}
\begin{align}
\boxed{
x_{A} = s - K_1 e^{K_2 z}
  }
\end{align}
```
---

## $x_A(z)$ Profile

```{=html}
<iframe width="100%" height="800"
		src="../../scripts/L03_xa_profile.html" title="Webpage example"></iframe>
```

--- 

## Notes on the Relation Between $N_A$ and $N_B$ (1)

Using steady state condition, we need to know relation between $N_A$ and $N_B$ *before* solving the general EQ.

It depends on the system setup and mass balance. 

Let's consider the same chemical reaction of hydrogen dissociation by a solid catalst

```{=tex}
\begin{align}
\text{H}_2\ (A, \text{gas}) \rightarrow 2\text{H}^*\ (B, \text{gas})
\end{align}
```

- Case 1: reaction through a solid catalyst at bottom of a tube

  - The flux of A and B have **opposite** signs
  - $N_B = -2 N_A$
  
## Notes on the Relation Between $N_A$ and $N_B$ (2)

- Case 2: gas flow through a solid catalyst inside a tube

  - The flux of A and B have the **same** sign
  - $N_B = 2 N_A$
  
Take home question: 
- How do the flux directions affect the general solution?

---

## Measuring Diffusivity $D_{AB}$ In Gases

- Several experimental methods exist for gases, evaporated liquid and sublimated solids (see *Geankoplis* Ch 6.2E)
- We will introduce the two-bulb method for gases
- Typical setup see Duncan & Toor *AIChE J.* 1962, 8, 38-41
- Which case should we apply?

---

## Two-Bulb Experiment: Conditions

Conditions for the two-bulb experiment

- Initially, pure A in bulb 1 and pure B and bulb 2
- $t=0$, the valve is opened slowly to minimize convection
- $t=t_e$, the valve is closed and the composition in 1 and 2 are analyzed
- The valve open time is much shorter than $t_2 - t_1$
- The tube is a very thin capillary üëâ no convection
- Constant $p_T$ and $T$ throughout experiment

---

## Two-Bulb Experiment: Pseudo Steady State

We can apply:

- EMCD condition (no convection)
- *Pseudo*-steady state (P.S.S) assumption
  - At each time step, we assume $N_A$ or $J_{Az}^*$ is constant (linear $c_A$ profile)
  - But net $N_A$ flux accumulates A molecules in bulb 2
  - $c_A$ in bulb 2 **changes** over time
  
--- 

## Two-Bulb Experiment: Governing Equations

We use the mass balance of the system

```{=tex}
\begin{align*}
\text{[Mass In]} &= \text{[Accumulation]} \\
S \cdot J_{Az}^* &= V_2 \frac{d c_{A2}}{dt} \\
D_{AB} \frac{c_{A1} - c_{A2}}{L} \cdot S &= V_2 \frac{d c_{A2}}{dt}
\end{align*}
```

Since the total pressure $p_T$ is constant, the average concentration of $c_A$ in the system, $c_{A, av}$ is also constant

```{=tex}
\begin{align*}
V_T c_{A, av} &= (V_1 + V_2)c_{A, av} \\
&= V_1c_{A1}(t=0) + V_2c_{A2}(t=0) \\
&= V_1c_{A1}(t\neq0) + V_2c_{A2}(t\neq0)
\end{align*}
```

---

## Two-Bulb Experiment: Solutions

We are interested in $c_{A2}$, so substitute $c_{A1}$ with relation to $c_{A, av}$:

$$
c_{A1} = \frac{V_T c_{A, av} - V_2 c_{A2}}{V_1}
$$

After the substitution, rearrangement and integration we get:

```{=tex}
\begin{align*}
\ln\!\left[
\frac{c_{A, av} - c_{A2}(t=t_e)}{c_{A, av} - c_{A2}(t=0)}
\right]
&= -\frac{D_{AB} V_T S}{V_1 V_2 L} \cdot t \\
\end{align*}
```

We can extract $D_{AB}$ usingt the slope of the plot!

---

## Some Typical Diffusivity Measurements

![](public/geankoplis-gas-diff){width=700}
^[Geankoplis Table 6.2-1]


---

## Summary

- General solution for $N_B = k N_A$
- Like stagnant B case, general solution take a **logarithm** form for $N_A$
- When $x_{A1}$ and $x_{A_2}$ are determined, the flux $N_A$ is controlled by the relation between $N_B$ and $N_A$
- The ratio between $N_B$ and $N_A$ depends on the system and setup
- Diffusivity $D_{AB}$ can be determined by EMCD through two-bulb setup

---

## Preview of Next Class: Theories for predicting $D_{AB}$

- Kinetic theory

$$
D_{AB} = \frac{1}{3} \overline{u} \lambda
$$

- Chapman-Enskog theory

$$
D_{AB} \propto \frac{T^{\frac{3}{2}}}{P} \left(\frac{1}{m_A} + \frac{1}{m_B} \right)^{\frac{1}{2}}
$$

- Fuller method

$$
D_{AB} \propto  \frac{T^{1.75}}{P} \left(\frac{1}{m_A} + \frac{1}{m_B} \right)^{\frac{1}{2}}
$$






